checkpoint on way to implementing TLB consistency tracking
 * vale procedures for STR and STRpte

 * added TLB invalidate and pushed secure mem preconditions through
   entry path as a test case

 * proved key lemmas about addresses in the page table given pageDbCorresponds

verified/kom_common.i.dfy
@@ -159,6 +159,11 @@ predicate NonStackMemPreserving(s:state, r:state)
     MemPreservingExcept(s, r, StackLimit(), StackBase())
 }
 
+predicate OnlySecureMemInPageTable(s:state)
+    requires ValidState(s)
+{
+    forall a:addr | AddrInPageTable(s, a) :: address_is_secure(a)
+}
 
 //-----------------------------------------------------------------------------
 // Common functions
